#ComputerScience  #IowaStateUniversity  #COMS331 
#Lecture

[[Classes/ISU/COM S 331/COM S 331]] [[2021-12-03]]

---

# COM S 331 Lecture 2021-12-03

 ## Regular Expressions (7-9)
 
 
 ### Def 
 
 Let $\sum$ be an alphabet. We define the regular expression $\alpha$ over $\sim$ and the languages $L(\alpha)$ that they denote by the following recursion. 
 
 - $\boldsymbol{\emptyset}$ , $\boldsymbol{\lambda}$ are regular expressions, with $L(\boldsymbol{\emptyset}) = \emptyset$ and $L(\boldsymbol{\lambda}) = \{\lambda\}$
 - For each $a \in \sum$ a is a regular expression, with $L(a) = \{a\}$
 - If $\alpha$ and $\beta$ are regular expressions, then so are $(\alpha + \beta), (\alpha \beta),$ and $(\alpha^*)$ with $L(\alpha + \beta)  L(\alpha) \cup L(\beta), L(\alpha  \beta) = L(\alpha) L(\beta) , L((\alpha)^*) = L(\alpha)^*$
 - Regular expressions $\alpha$ and $\beta$ are equivalent, and we write $\alpha \equiv \beta$ of $L(\alpha) = L(\beta)$

Some algebraic laws (easily verified) that can be used to simplify regular expressions
- $(9.1)$ $\alpha + (\beta + \gamma) \equiv (\alpha + \beta) + \gamma$ (associative +)
- $(9.2)$ $\alpha + \beta \equiv \beta + \alpha$ (comm +)
- $(9.3)$ $\alpha + \boldsymbol{\emptyset} \equiv \alpha$
- $(9.4)$ $\alpha +\alpha \equiv \alpha$
- $(9.5)$ $\alpha(\beta \gamma) \equiv (\alpha \beta) \gamma$
- $(9.6)$ $\boldsymbol{\lambda} \alpha \equiv \boldsymbol{\lambda} \equiv \alpha$
- $(9.7)$ $\alpha(\beta + \gamma) \equiv \alpha\beta + \alpha \gamma$
- $(9.8)$ $(\alpha + \beta) \gamma \equiv \alpha \gamma + \beta \gamma$
- $(9.9)$ $\emptyset \alpha \equiv \alpha \boldsymbol{\emptyset} \equiv \emptyset$
- $(9.10)$ $\lambda + \alpha \alpha^*  \equiv \alpha^*$
- $(9.11)$ $\boldsymbol{\lambda} + \alpha^* \alpha \equiv \alpha^*$

Notation $\alpha \leq \beta$ means that $L(\alpha) \subseteq L(\beta)$

Remark $\alpha \leq \beta \Leftrightarrow L(\alpha) \subseteq L(\beta)$

$\Leftrightarrow L(\alpha) \cup  L(\beta) = L(\beta)$
$\Leftrightarrow \alpha + \beta = \beta$

Two more lemmas that are useful 

- $(9.12)$ $\beta + \alpha \gamma  \leq \gamma \Rightarrow \alpha^* \beta \leq \gamma$
- $(9.13)$ $\beta + \gamma \alpha \leq \gamma \Rightarrow \beta \alpha^* \leq \gamma$

Fact (Kozen '94) Laws (9.1) - (9.13) are sufficient to give algebraic proofs of all true equations concerning regular expressions.
