#ComputerScience  #IowaStateUniversity  #COMS331 
#Lecture

[[COM S 331]] [[2021-11-19]]

---

# COM S 331 Lecture 2021-11-19

## Theorem. 

For every NFA N there is a DFA M such that $L(M) = L(N)$

### Proof 

Let $N = (Q, \sum, \Delta, S, F)$ be an NFA
Define the DFA $M = (\mathbb{P}(Q)m \sum, \delta, s, \mathbb{F})$

by $s = S;$
$\mathbb{F} = \{A \subseteq Q | A \cap F \not= \emptyset\}$,
$\delta : \mathbb{P}(Q) \times \sum \rightarrow \mathbb{P}(Q)$
$\delta(A,a) = \Delta(A,a)$.

To prove that $L(M) - M(N)$, we use the following two lemmas from the text, both of which are proven by routine induction 

Lemma 6.1 If $N = (Q, \sum, \Delta, S, F)$ is an NFA , $x, y \in \sum^*$ and $A \subseteq Q$, then
$\hat{\Delta}(A, xy) = \hat{\Delta}(\hat{\Delta}(A,x), y)$

Lemma 6.2: If $N = (Q, \sum, \Delta, S, F)$ is an NFA, then $\hat{\Delta}$ computes with set union. That is for any family $\mathbb{F}$ of subsets Q any $x \in \sum^*$, 

$\hat{\Delta}(\cup \mathbb{F}, x)= \bigcup\limits_{A \in \mathbb{F}}{} \hat{\Delta}(A,x)$


The key part of the proof that $L(M) = L(N)$ is the following.

***claim*** For all $A \in \mathbb{P}(Q)$ and $x \in \sum^*$, $\hat{\delta}(A,x) = \hat{\Delta}(A,x)$

Assume for a moment that the claim is true. 

Thus, for all $x \in \sum^*$, 

$x \in L(M) \overset{\text{DFA semantics}}{\Leftrightarrow} \hat{\delta}(s,x) \in \mathbb{F}$
$\Leftrightarrow \hat{\delta}(S,x) \in \mathbb{F}$
$\overset{\text{Claim}}{\Leftrightarrow} \hat{\Delta}(S,x) \in \mathbb{F}$
$\overset{\text{def}\ \mathbb{F}}{\Leftrightarrow} \hat{\Delta}(S,x) \cap F \not= \emptyset$
$\overset{\text{NFA Semantics}}{\Leftrightarrow}$ N accepts x
$\Leftrightarrow x \in L(N)$
so $L(M) =L(N)$.

So it suffices to prove the claim. we do this by induction on x.


- $\hat{S}(S,\lambda) \overset{\text{def}\ \hat{\delta}}{=} A \overset{def \hat{\Delta}}{=}\hat{\Delta}(A,\lambda)$
- Assume that the claim holds for x, where $x\in \sum^*$, and let $a \in \sum$, Then 

$\hat{\delta}(A,xa) \overset{def \hat \ {\delta}}{=} \delta(\hat{\delta}(A,x),a)$
$\overset{induction\ hyp}{=} \delta(\hat{\Delta}(A,x),a)$

$\overset{def\ \delta}{=} \hat{\Delta}(\hat{\Delta}(A,x),a)$
$\overset{\text{Lemma 6-1}}{=}\hat{\Delta}(A, xa)$ $\blacksquare$

---

$A \subseteq \{0,1\}^*$ is regular
$A' = \{x \in \{0,1\}^* | \text{x is within 3 bit-flips of some string} y \in A\}$

$\therefore A'$ is regular

---

## recall

That we defined, for each $k \in \mathbb{Z}^+$, the language $A_k = \{x \in \{0,1\}^* | \text{the kth to last bit of x is 1}\}$

***claim*** Every DFA that decides $A_K$ has $\geq 2^k$ states. (we saw how to do with a (k + a) state NFA)
### Proof
Let $M = (Q, \sum, \delta, s, F)$ be a DFA with $|Q| < 2^k$

It suffices to show that $L(M) \not= A_k$.

Since $|Q| < 2^k = |\{0,1\}^k|$, there exists $x,y \in \{0,1\}^k$ such that $x \not= y$ and $\hat{\delta}(s,x) = \hat{\delta}(s, y)$. 

Since $x \not = y$, there exists $u,v,w \in \{0,1\}^*$ and $b \in \{0,1\}$ such that 

$x = ubv $ and $y = u\overline{b}w$,
where $\overline{b} = 1 - b$. Note that $0 \leq |u| < k$
and $|v| = |w| = k - |u| - 1$. Let 
$x' = xu$ and $y' = yu$

Then 

$x' = ubvu\ $, $y' = u\overline{b}wu$
and $|vu| = |wu| = k-1$, so the kth to last bits of x' and y' are b and $\overline{b}$, respectively. 

it follows that exactly one of $x'$ and $y'$ is an element of $A_k$.

However,

$\hat{\delta}(s,x')= \hat{\delta}(s,xu)$
$\overset{hw}{=}\hat{\delta}(\hat{\delta}(s,x),u)$
$\overset{}{=}\hat{\delta}(\hat{\delta}(s,y),u)$
$\overset{hw}{=}\hat{\delta}(s,yu)$
$= \hat{\delta}(s,y')$

So M accepts both or neither of x', y'

Hence $L(M) \not = A_k$ $\blacksquare$