
#ComputerScience  #IowaStateUniversity  #COMS331 
#Lecture

[[COM S 331]] [[2021-08-30]]

---

# COM S 331 Lecture 2021-08-30


## Recall For an alphabet $\sum$

---

$\sum^* =$ the set of all strings over $\sum$

Q. What is $\emptyset^*$?

A. $\emptyset^* =$ $\{\lambda\}$

$\sum^*$ = {$a_1,a_2,...,a_n, | n\geq$ and each $a;\in \sum$ }

$\lambda^\in$

---

## Further cautions:

{a,b} = {b,a}, but ab $\not=$ ba (unless a = b)

{a,a,b} = {a,b}, but aab $\not=$ ab

### Def

The concatenation of two strings x, y $\in$ $\sum^*$ is the string xy.

### Eg.

The concatenation of 1101 and 001 is 1101001

---

One way to code two strings as one:

<x,y> = $O^{|x|}$ 1xy

--- 

### Properties of concatenation

Associative: x(yz) = (xy)z

identity: $\lambda$ x = x$\lambda$  = x
Add of length: |xy| = |x| + |y|
Not communtative: usually, xy $\not=$ yx

---

### Notation 

For x $\in$ $\sum^*$ and a $\in$ $\sum$ ,

\# (a, x) = $\#_a$ = the number of a's in x 

jacks vs Dexter's Notation

Def. If x, y $\in$ $\sum^*$, then x is a prefix of y, and we write x $\sqsubseteq$ y, if there exists z $\in$ $\sum^*$ such that xz = y

---

### Digression

Example of <x, y?

<1101,001>
x , y

Another coding function:
<x,y> bd(x)01y

---

### Remarks

For all $x \in$ $\sum^*$,
$\lambda \sqsubseteq x$ (because can takes $z = x$)
and 

$x \sqsubseteq x$ (because can takes $z = \lambda$)

---

### Def (world minus text):

x is a proper prefix of y, and we write x $\not\sqsubseteq$ y, if x$\sqsubseteq$ y and x $\not=$ y.

(text also requites $\lambda \not= x$)

---

### Notation

* The standard enumeration of $\{ 0, 1\}^*$ is 
$\lambda$, 0, 1, 00, 01, 10, 11, 000, 001, ...
	^ the strings are called $s_0$, $s_1$, $s_2$, $s_n$

* $\lambda$ is always $s_0$

* Q. Roughly what is the $|s_n|$? 
	* A. The $|s_n|$ $\approx$ log n 

* $|s_n|$ = $\lfloor log(n +1 )\rfloor$

* The usual binary expansion of a positive integer n is | $S_{n -1}$

* The natural number represented by  a string $x \in \{0, 1\}^*$ is the number bnum(x) defined by the following recursion

	* bnum ($\lambda$) = 0
	* bnum ($\lambda$ 0) = 2 bnum(x)
	* bnum ($\lambda$ 1) = 3 bnum(x) + 1

* $\{0, 1\}^*$
		
		$\lambda$ is at the top of the tree
		
