#ComputerScience  #IowaStateUniversity  #COMS331 
#Lecture

[[COM S 331]] [[2021-12-06]]

---

# COM S 331 Lecture 2021-12-06

## Recall

- Kozen '94 (9.1) - (9.13) suffices to give algebraic proofs of all true equations involving regular expressions



## Five useful equations 

- (9.14) $(\alpha \beta)^* \alpha = \alpha(\beta \alpha)^*$
- (9.15) $(\alpha^* \beta)^* \alpha^* = (\alpha + \beta)^*$
- (9.16) $\alpha^*(\beta \alpha^*)^* = (\alpha + \beta)^*$
- (9.17) $(\lambda + \alpha)^* \equiv \alpha^*$
- (9.18) $\alpha \alpha^* \equiv \alpha^* \alpha$


## Notation 

If k = 0, then 

$\alpha_1 + \alpha_2 + ... + \alpha_k$ = $\emptyset$

## Example 

An algebraic proof of (9.14) that illustrates the power of (9.12)

(9.12) -> $\beta + \alpha + \gamma \Rightarrow \alpha^* \beta \leq \gamma$

### Claim 1

$(\alpha \beta)^* \alpha \leq \alpha(\beta \alpha)^*$

### Proof 1

By (9.12), it suffices to show that 

$\alpha + \alpha \beta \alpha(\beta \alpha)^* \leq \alpha(\beta \alpha)^*$

well, 

$\alpha + \alpha \beta \alpha(\beta \alpha)^* + \alpha(\beta \alpha)^*$

$\overset{(9.7)}{\equiv} \alpha(\lambda + \beta \alpha(\beta \alpha)^* + (\beta \alpha)^*$
$\overset{(9.10)}{\equiv} \alpha ((\beta \alpha)^* + (\beta \alpha)^*)$
$\overset{(9.4)}{\equiv} \alpha(\beta \alpha)^*$ $\blacksquare$ for claim 1

### Claim 2 

The next goal is to see why the languages represented by regular expressions are exactly the regular languages 

First sketch: regular exp => reg

### Lemma A

If $A, B \subseteq \sum^*$ are regular, then so is $AB$.

### Proof A 

Assume the hypothesis. Then there exists NFAs 

$N_A = (Q_A, \sum, \Delta_A, s_A, F_A)$,
$N_B = (Q_B, \sum, \Delta_B, s_B, F_B)$

such that $L(N_A) = A$ and $L(N_B)= B$.

we can assume, renaming states as necessary, that $Q_A \cap Q_B = \emptyset$

Define the NFA

$N = (Q_A \cup Q_B, \sum, \Delta, s_A, F_B)$

Where 

$\Delta : (Q_A \cup Q_B) \times \sum \rightarrow \mathbb{P}(Q_A \cup Q_B)$

is defined by 

$\Delta(q, a) =\{$

- $\Delta_B(q,a)$ ... if $q \in Q_B$
- $\Delta_A(q,a)$ ... if $q \in Q_A$ and $\Delta_A (q,a) \cap F_A = \emptyset$
-  $\Delta_A(q,a) \cup S_B$ ...  if $q \in Q_A$ and $\Delta_A(q,a) \cap F_A \not= \emptyset$


Routine if tedious to see that this works $\blacksquare$

### Lemma B

If $A \subseteq \sum^*$ is regular, then so is $A^+$.

### Proof B

Similar thinking, with a loop to lemma A $\blacksquare$

### Corollary C

If $A \subseteq \sum^*$ is regular, then $A^*$ is regular. 

### Proof  C

$A^* = A^+ \cup \{\lambda\}$

- $A^+$ is reg by Claim B
- $\{\lambda\} reg by NFA$
- $A^+ \cup \{\lambda\}$ by closure under $\cup$

$\blacksquare$

